State -> Option Store

MasterThesis/SCORE/Interpreter.lean
@@ -3,53 +3,53 @@ import Mathlib.Logic.Function.Iterate
 
 namespace SCORE
 
-open SCORE.State SCORE.Com
+open SCORE Com
 
 mutual
   def eval (P : Com) (s : State) : State :=
     match s with
-    | fail   => fail
-    | prog σ =>
+    | none   => none
+    | some σ =>
       match P with
       | SKIP    => s
-      | CON x   => prog ([x ↦ (0 :: (σ x))] σ)
+      | CON x   => some ([x ↦ (0 :: (σ x))] σ)
       | NOC x   => match (σ x).head? with
-                   | some 0 => prog ([x ↦ (σ x).tail] σ)
-                   | _      => fail
+                   | some 0 => some ([x ↦ (σ x).tail] σ)
+                   | _      => none
       | DEC x   => match (σ x).head? with
-                   | some v => prog ([x ↦ ((v - 1) :: (σ x).tail)] σ)
-                   | none   => fail
+                   | some v => some ([x ↦ ((v - 1) :: (σ x).tail)] σ)
+                   | none   => none
       | INC x   => match (σ x).head? with
-                   | some v => prog ([x ↦ ((v + 1) :: (σ x).tail)] σ)
-                   | none   => fail
+                   | some v => some ([x ↦ ((v + 1) :: (σ x).tail)] σ)
+                   | none   => none
       | SEQ P Q => (eval Q) (eval P s)
       | FOR x P => match (σ x).head? with
                    | some v => match v with
                                | Int.ofNat   k => (fun τ => eval  P τ)^[k] s
                                | Int.negSucc k => (fun τ => evalI P τ)^[k.succ] s
-                   | none   => fail
+                   | none   => none
   def evalI (P : Com) (s : State) : State :=
     match s with
-    | fail   => fail
-    | prog σ =>
+    | none   => none
+    | some σ =>
       match P with
       | SKIP    => s
       | CON x   => match (σ x).head? with
-                   | some 0 => prog ([x ↦ (σ x).tail] σ)
-                   | _   => fail
-      | NOC x   => prog ([x ↦ (0 :: (σ x))] σ)
+                   | some 0 => some ([x ↦ (σ x).tail] σ)
+                   | _   => none
+      | NOC x   => some ([x ↦ (0 :: (σ x))] σ)
       | DEC x   => match (σ x).head? with
-                   | some v => prog ([x ↦ ((v + 1) :: (σ x).tail)] σ)
-                   | none   => fail
+                   | some v => some ([x ↦ ((v + 1) :: (σ x).tail)] σ)
+                   | none   => none
       | INC x   => match (σ x).head? with
-                   | some v => prog ([x ↦ ((v - 1) :: (σ x).tail)] σ)
-                   | none   => fail
+                   | some v => some ([x ↦ ((v - 1) :: (σ x).tail)] σ)
+                   | none   => none
       | SEQ P Q => (evalI Q) (evalI P s)
       | FOR x P => match (σ x).head? with
                    | some v => match v with
                                | Int.ofNat   k => (fun τ => evalI P τ)^[k] s
                                | Int.negSucc k => (fun τ => eval  P τ)^[k.succ] s
-                   | none   => fail
+                   | none   => none
 end
 
 end SCORE
